Util/TransUtil.v
@@ -1,3 +1,5 @@
+Require Import Coq.Program.Equality.
+
 Inductive Steps_ {Ev State} 
     (step : State -> Ev -> State -> Prop) 
     (st : State) :
@@ -11,12 +13,62 @@ Inductive Steps_ {Ev State}
 Definition Steps {Ev State} (step : State -> Ev -> State -> Prop) st evs st' 
     := Steps_ step st evs st'.
 
-Lemma Steps_nil {E A} (step : A -> E -> A -> Prop) x y
-  : Steps step x nil y <-> x = y.
-Proof.
-  split.
-  - inversion 1; auto.
-  - intros []; constructor.
+Inductive bwd_list {A} :=
+| Start
+| Snoc (xs : bwd_list) (x : A).
+Arguments bwd_list : clear implicits.
+
+Fixpoint bwd_app {A} (xs ys : bwd_list A) : bwd_list A :=
+  match ys with
+  | Start => xs
+  | Snoc ys y => Snoc (bwd_app xs ys) y
+  end.
+
+Inductive BwdSteps {Ev State} 
+    (step : State -> Ev -> State -> Prop) 
+    (st : State) :
+    bwd_list Ev -> 
+    State 
+    -> Prop :=
+| BwdStepsNone : BwdSteps step st Start st
+| BwdStepsMore ev evs st' st'' :
+    BwdSteps step st evs st' ->
+    step st' ev st'' ->
+    BwdSteps step st (Snoc evs ev) st''
+.
+
+
+
+Fixpoint to_bwd {A} (xs : list A) : bwd_list A :=
+  match xs with
+  | nil => Start
+  | cons x ys => bwd_app (Snoc Start x) (to_bwd ys)
+  end.
+
+Fixpoint from_bwd {A} (xs : bwd_list A) : list A :=
+  match xs with
+  | Start => nil
+  | Snoc ys x => app (from_bwd ys) (cons x nil)
+  end.
+
+Lemma to_bwd_nil {A} (xs : list A) :
+  Start = to_bwd xs ->
+  xs = nil.
+intros.
+induction xs.
+easy.
+simpl in *.
+Admitted.
+
+Lemma BwdSteps_app {E A} (step : A -> E -> A -> Prop) (xs ys : bwd_list E) s s' s''
+  : BwdSteps step s xs s' -> BwdSteps step s' ys s'' -> BwdSteps step s  (bwd_app xs ys) s''.
+intros.
+induction H0.
+easy.
+simpl.
+econstructor.
+exact IHBwdSteps.
+easy.
 Qed.
 
 Lemma Steps_app {E A} (step : A -> E -> A -> Prop) (xs ys : list E) s s' s''
@@ -25,6 +77,43 @@ Proof.
   unfold Steps.
   induction 1; cbn; auto.
   econstructor; eauto.
+Qed.
+
+Lemma Steps_iso {Ev State} {step : State -> Ev -> State -> Prop} (st st' : State) (xs : list Ev) :
+  Steps step st xs st' ->
+  BwdSteps step st (to_bwd xs) st'.
+generalize dependent st'.
+generalize dependent st.
+generalize dependent xs.
+fix rec 4.
+intros.
+destruct H.
+constructor.
+simpl.
+eapply BwdSteps_app.
+econstructor.
+constructor.
+exact H.
+apply rec.
+easy.
+Qed.
+
+Lemma BwdSteps_iso {Ev State} {step : State -> Ev -> State -> Prop} (st st' : State) (xs : list Ev) :
+  BwdSteps step st (to_bwd xs) st' ->
+  Steps step st xs st'.
+generalize dependent st'.
+generalize dependent st.
+generalize dependent xs.
+fix rec 4.
+intros.
+Admitted.
+
+Lemma Steps_nil {E A} (step : A -> E -> A -> Prop) x y
+  : Steps step x nil y <-> x = y.
+Proof.
+  split.
+  - inversion 1; auto.
+  - intros []; constructor.
 Qed.
 
 Inductive PointStep {Index Ev State : Type} (step : State -> Ev -> State -> Prop)
