Core/RefinesFacts.v
@@ -7,6 +7,7 @@ From LHL.Core Require Import
   Program
   Specs
   Traces
+  TracesFacts
   Eutt.
 
 From Coq Require Import
@@ -34,21 +35,52 @@ Theorem eutt_layerRefines {E F} :
   forall (spec : Spec E) (impl impl' : Impl E F), 
   euttImpl ieq impl impl' -> 
   layerRefines (spec :> impl) (spec :> impl').
+unfold euttImpl, layerRefines, specRefines, Incl, IsTraceOfSpec, Steps.
 Admitted.
-
-(* Lemma foo {E F} {spec : Spec F} {impl : Impl E F} p :
-  IsTraceOfSpec p (overObj (spec :> impl)) ->
-  IsTraceOfSpec p spec. *)
 
 (* Crucial Refinement Properties *)
 
+Lemma help {E F} :
+  forall (p : Trace (ThreadLEvent E F)),
+  projSilent (projUnder p) = projUnderThr p.
+intros.
+induction p.
+easy.
+destruct a, l, ev.
+simpl.
+rewrite IHp.
+all: easy.
+Qed.
+
 Theorem mkLayer_monotonic {E F} :
-  forall (spec : Spec E) (spec' : Spec E) (impl : Impl E F),
+  forall (spec spec' : Spec E) (impl : Impl E F),
   specRefines spec' spec -> 
   layerRefines (spec' :> impl) (spec :> impl).
 unfold layerRefines, specRefines, Incl, IsTraceOfSpec.
 intros.
-Admitted.
+destruct_all.
+apply overObj_iso in H0.
+destruct_all.
+subst.
+rewrite decompInterSteps in H1.
+destruct_all.
+rewrite decompUnderSteps in H1.
+destruct_all.
+eassert (exists st, Steps _ _ _ st).
+exists (snd x).
+exact H1.
+apply H in H3. clear H.
+destruct_all.
+exists (fst x, x1).
+apply InterSteps_iso.
+simpl in *.
+rewrite decompInterSteps.
+split.
+exact H0.
+rewrite decompUnderSteps.
+simpl.
+easy.
+Qed.
 
 Theorem layerRefines_VComp_assoc {E F G} : 
   forall  (spec : Spec E) (impl : Impl E F) (impl' : Impl F G),
